Finish typing_leq_term proof

pcuic/theories/PCUICElimination.v
@@ -23,6 +23,27 @@ Proof.
   rewrite H in H1. inversion H1. subst. rewrite H2 in H0. inversion H0. eauto.
 Qed.
 
+Lemma declared_constructor_inj `{cf : checker_flags} {Σ mdecl mdecl' idecl idecl' cdecl cdecl' c} :
+  declared_constructor Σ mdecl' idecl' c cdecl ->
+  declared_constructor Σ mdecl idecl c cdecl' ->
+  mdecl = mdecl' /\ idecl = idecl'  /\ cdecl = cdecl'.
+Proof.
+  intros [] []. 
+  destruct (declared_inductive_inj H H1); subst.
+  rewrite H0 in H2. noconf H2. intuition congruence.
+Qed.
+
+Lemma declared_projection_inj `{cf : checker_flags} {Σ mdecl mdecl' idecl idecl' pdecl pdecl' p} :
+  declared_projection Σ mdecl' idecl' p pdecl ->
+  declared_projection Σ mdecl idecl p pdecl' ->
+  mdecl = mdecl' /\ idecl = idecl'  /\ pdecl = pdecl'.
+Proof.
+  intros [] []. 
+  destruct (declared_inductive_inj H H1); subst.
+  destruct H0, H2.
+  rewrite H0 in H2. noconf H2. intuition congruence.
+Qed.
+
 Definition SingletonProp `{cf : checker_flags} (Σ : global_env_ext) (ind : inductive) :=
   forall mdecl idecl,
     declared_inductive (fst Σ) mdecl ind idecl ->
@@ -193,6 +214,8 @@ Inductive All_local_assum (P : context -> term -> Type) : context -> Type :=
 | localassum_cons_def Γ na b t :
     All_local_assum P Γ ->
     All_local_assum P (Γ ,, vdef na b t).
+
+Derive Signature for All_local_assum.
 
 Lemma All_local_assum_app P Γ Δ : All_local_assum P (Γ ++ Δ) ->
   All_local_assum P Δ *
@@ -618,6 +641,48 @@ Proof.
   todo "Simon"%string.
 Qed.
 
+Lemma principal_type_ind {Σ Γ c ind u u' args args'} {wfΣ: wf Σ.1} :
+  Σ ;;; Γ |- c : mkApps (tInd ind u) args ->
+  Σ ;;; Γ |- c : mkApps (tInd ind u') args' ->
+  PCUICEquality.R_universe_instance (eq_universe (global_ext_constraints Σ)) u u' * 
+  All2 (conv Σ Γ) args args'.
+Proof.
+  intros h h'.
+  destruct (principal_typing _ wfΣ h h') as [C [l [r ty]]].
+  eapply invert_cumul_ind_r in l as [ui' [l' [red [Ru eqargs]]]]; auto.
+  eapply invert_cumul_ind_r in r as [ui'' [l'' [red' [Ru' eqargs']]]]; auto.
+  destruct (red_confluence wfΣ red red') as [nf [redl redr]].
+  eapply red_mkApps_tInd in redl as [args'' [-> eq0]]; auto.
+  eapply red_mkApps_tInd in redr as [args''' [eqnf eq1]]; auto.
+  solve_discr.
+  split. transitivity ui'; eauto. now symmetry.
+  eapply All2_trans; [|eapply eqargs|]. intro; intros. eapply conv_trans; eauto.
+  eapply All2_trans. intro; intros. eapply conv_trans; eauto.
+  2:{ eapply All2_sym. eapply (All2_impl eqargs'). intros. now apply conv_sym. }
+  eapply All2_trans. intro; intros. eapply conv_trans; eauto.
+  eapply (All2_impl eq0). intros. now apply red_conv.
+  eapply All2_sym; eapply (All2_impl eq1). intros. symmetry. now apply red_conv.
+Qed.
+
+Definition projection_context mdecl idecl ind := 
+  smash_context [] (PCUICEnvironment.ind_params mdecl),,
+       PCUICEnvironment.vass (nNamed (PCUICEnvironment.ind_name idecl))
+         (mkApps
+            (tInd
+               {|
+               inductive_mind := inductive_mind ind;
+               inductive_ind := inductive_ind ind |}
+               (polymorphic_instance (PCUICEnvironment.ind_universes mdecl)))
+            (PCUICEnvironment.to_extended_list
+               (smash_context [] (PCUICEnvironment.ind_params mdecl)))).
+
+Lemma projection_subslet Σ Γ mdecl idecl ind u c args : 
+  Σ ;;; Γ |- c : mkApps (tInd ind u) args ->
+  subslet Σ Γ (c :: List.rev args) (projection_context mdecl idecl ind). 
+Proof.
+  todo "Projections"%string.
+Qed.
+
 Lemma typing_leq_term (Σ : global_env_ext) Γ t t' T T' : 
   wf Σ.1 ->
   Σ ;;; Γ |- t : T ->
@@ -659,7 +724,168 @@ Proof.
     eapply context_conversion; eauto.
     constructor; pcuic. constructor. symmetry;  now constructor.
     constructor; pcuic.
-Admitted.    
+
+  - eapply inversion_Lambda in X4 as (s & B & dom & codom & cum); auto.
+    specialize (X1 _ _ dom (PCUICEquality.eq_term_leq_term _ _ _ X5_1)).
+    assert(conv_context Σ (Γ ,, vass na ty) (Γ ,, vass n t)).
+    { repeat constructor; pcuic. }
+    specialize (X3 t0 B).
+    forward X3 by eapply context_conversion; eauto; pcuic.
+    econstructor.
+    econstructor. eauto. instantiate (1 := bty).
+    eapply context_conversion; eauto; pcuic.
+    constructor; pcuic. constructor; pcuic. symmetry; constructor; auto.
+    have tyl := type_Lambda _ _ _ _ _ _ _ X0 X2.
+    now eapply PCUICValidity.validity in tyl.
+    eapply congr_cumul_prod; eauto.
+    constructor; auto. reflexivity.
+    
+  - eapply inversion_LetIn in X6 as (s1' & A & dom & bod & codom & cum); auto.
+    specialize (X1 _ _ dom (PCUICEquality.eq_term_leq_term _ _ _ X7_2)).
+    specialize (X3 _ _ bod (PCUICEquality.eq_term_leq_term _ _ _ X7_1)).
+    assert(conv_context Σ (Γ ,, vdef na t ty) (Γ ,, vdef n b b_ty)).
+    { repeat constructor; pcuic. }
+    specialize (X5 u A).
+    forward X5 by eapply context_conversion; eauto; pcuic.
+    specialize (X5 X7_3).
+    econstructor.
+    econstructor. eauto. eauto.
+    instantiate (1 := b'_ty).
+    eapply context_conversion; eauto.
+    apply conv_context_sym; auto.
+    pcuic. eapply PCUICValidity.validity; eauto.
+    econstructor; eauto.
+    eapply cum_LetIn; pcuic.
+    
+  - eapply inversion_App in X4 as (na' & A' & B' & hf & ha & cum); auto.
+    specialize (X1 _ _ hf X5_1).
+    specialize (X3 _ _ ha (PCUICEquality.eq_term_leq_term _ _ _ X5_2)).
+    econstructor.
+    econstructor; [eapply X1|eapply X3].
+    eapply PCUICValidity.validity; pcuic.
+    eapply type_App; eauto.
+    eapply conv_cumul. eapply (subst_conv Γ [vass na A] [vass na A] []); pcuic.
+    repeat constructor. now rewrite subst_empty.
+    repeat constructor. now rewrite subst_empty.
+    eapply PCUICValidity.validity in X0; auto.
+    apply PCUICArities.isWAT_tProd in X0 as [tyA]; auto.
+    constructor; auto.
+
+  - eapply inversion_Const in X1 as [decl' [wf [declc [cu cum]]]]; auto.
+    econstructor; eauto.
+    econstructor; eauto.
+    eapply PCUICValidity.validity; eauto.
+    econstructor; eauto.
+    eapply conv_cumul. constructor.
+    pose proof (declared_constant_inj _ _ H declc); subst decl'.
+    eapply eq_term_upto_univ_subst_instance_constr; eauto; typeclasses eauto.
+  
+  - eapply inversion_Ind in X1 as [decl' [idecl' [wf [declc [cu cum]]]]]; auto.
+    econstructor; eauto.
+    econstructor; eauto.
+    eapply PCUICValidity.validity; eauto.
+    econstructor; eauto.
+    eapply conv_cumul. constructor.
+    pose proof (declared_inductive_inj isdecl declc) as [-> ->].
+    eapply eq_term_upto_univ_subst_instance_constr; eauto; typeclasses eauto.
+  
+  - eapply inversion_Construct in X1 as [decl' [idecl' [cdecl' [wf [declc [cu cum]]]]]]; auto.
+    econstructor; eauto.
+    econstructor; eauto.
+    eapply PCUICValidity.validity; eauto.
+    econstructor; eauto.
+    pose proof (declared_constructor_inj isdecl declc) as [-> [-> ->]].
+    unfold type_of_constructor.
+    transitivity (subst0 (inds (inductive_mind (ind, i).1) u (ind_bodies mdecl))
+    (subst_instance_constr u0 cdecl'.1.2)).
+    * eapply conv_cumul.
+      eapply (conv_subst_conv _ Γ _ _ []); eauto.
+      { unfold inds.
+        generalize #|ind_bodies mdecl|.
+        induction n; simpl; constructor; auto.
+        constructor. constructor. auto. }
+      eapply subslet_untyped_subslet.
+      eapply (weaken_subslet _ _ _ Γ []); eauto.
+      eapply PCUICArities.subslet_inds; eauto.
+      destruct declc; eauto.
+      eapply subslet_untyped_subslet.
+      eapply (weaken_subslet _ _ _ Γ []); eauto.
+      eapply PCUICArities.subslet_inds; eauto.
+      destruct declc; eauto.
+    * constructor. eapply PCUICEquality.subst_leq_term.
+      eapply PCUICEquality.eq_term_leq_term.
+      eapply eq_term_upto_univ_subst_instance_constr; eauto; typeclasses eauto.
+
+  - eapply inversion_Case in X6 as (u' & args' & mdecl' & idecl' & ps' & pty' & btys' & inv); auto.
+    intuition auto.
+    intuition auto.
+    eapply type_Cumul.
+    econstructor; eauto.
+    eapply PCUICValidity.validity; eauto.
+    eapply (type_Case _ _ (ind, npar)). eapply isdecl.
+    all:eauto.
+    eapply (All2_impl X5); firstorder.
+    eapply conv_cumul.
+    eapply mkApps_conv_args; pcuic.
+    eapply All2_app. simpl in *.
+    2:constructor; pcuic.
+    eapply All2_skipn.
+    clear -wfΣ a5 X4 X7_2.
+    specialize (X4 _ _ a5 (PCUICEquality.eq_term_leq_term _ _ _ X7_2)).
+    eapply (principal_type_ind a5 X4).
+    
+  - eapply inversion_Proj in X3 as (u' & mdecl' & idecl' & pdecl' & args' & inv); auto.
+    intuition auto.
+    eapply type_Cumul.
+    econstructor; eauto.
+    eapply PCUICValidity.validity; eauto.
+    eapply type_Proj; eauto.
+    specialize (X2 _ _ a0 (PCUICEquality.eq_term_leq_term _ _ _ X4)).
+    pose proof (principal_type_ind X2 a0) as [Ruu' X3].
+    transitivity (subst0 (c :: List.rev args) (subst_instance_constr u' pdecl'.2)).
+    eapply conv_cumul.
+    destruct (on_declared_projection wfΣ a) as [[oni oib] onp].
+    destruct p as [[ind n] k].
+    red in onp. simpl in onp.
+    match goal with 
+    [ _ : on_type _ _ ?Γ _ |- _ ] => set(ctx := Γ) in *
+    end.
+    eapply (conv_subst_conv _ Γ ctx ctx []); eauto.
+    constructor. now constructor.
+    eapply All2_rev. apply All2_sym. apply (All2_impl X3). intros; now symmetry.
+    eapply subslet_untyped_subslet; eauto.
+    eapply projection_subslet; eauto.
+    eapply subslet_untyped_subslet; eauto.
+    eapply projection_subslet; eauto.
+    constructor. eapply PCUICEquality.subst_leq_term.
+    destruct (declared_projection_inj a isdecl) as [<- [<- <-]].
+    subst ty.
+    eapply PCUICEquality.eq_term_leq_term.
+    eapply eq_term_upto_univ_subst_instance_constr; eauto; try typeclasses eauto.
+    now symmetry.
+
+  - eapply inversion_Fix in X2 as (decl' & fixguard' & Hnth & types' & bodies & cum); auto.
+    eapply type_Cumul.
+    econstructor; eauto.
+    eapply PCUICValidity.validity; eauto.
+    econstructor. 2:eapply H0. all:eauto.
+    eapply (All_impl X0); firstorder.
+    eapply (All_impl X1); firstorder.
+    eapply All2_nth_error in a; eauto.
+    destruct a as [[eqty _] _].
+    constructor. now apply PCUICEquality.eq_term_leq_term.
+  
+  - eapply inversion_CoFix in X2 as (decl' & fixguard' & Hnth & types' & bodies & cum); auto.
+    eapply type_Cumul.
+    econstructor; eauto.
+    eapply PCUICValidity.validity; eauto.
+    eapply type_CoFix. 2:eapply H. all:eauto.
+    eapply (All_impl X0); firstorder.
+    eapply (All_impl X1); firstorder.
+    eapply All2_nth_error in a; eauto.
+    destruct a as [[eqty _] _].
+    constructor. now apply PCUICEquality.eq_term_leq_term.
+Qed.
 
 Lemma leq_prop_is_prop {Σ x s} : leq_universe Σ x s -> 
   (Universe.is_prop s <-> Universe.is_prop x).
